s

c-test/main.c
@@ -8,10 +8,17 @@ int abs(int x) {
         return -x;
     return x;
 }
+int square(int x) {
+    return x*x;
+}
 
 int main(void) {
     int values[] = { -10, -1, 0, 1, 42 };
     int n = sizeof(values) / sizeof(values[0]);
+    
+    int n_square = square(5);
+    
+    printf("square of 5 is %d\n", n_square);
 
     printf("Testing abs():\n");
 
