c-test/c-test.lean
@@ -11,3 +11,10 @@ theorem abs_correct (x : Int) :
   absImpl x = absSpec x := by
   unfold absImpl absSpec
   rfl
+def add_32 (a b : Int32) : Int32 := a + b
+
+#eval add_32 5 4
+
+def square (x : Int) : Int :=
+  x * x
+theorem square_correct (x : Int) :
